clean up

theories/approxis/examples/advantage.v
@@ -1,7 +1,8 @@
 From clutch.approxis Require Import approxis.
 From clutch.approxis Require Export bounded_oracle.
-From Coquelicot Require Import Lub.
 Set Default Proof Using "Type*".
+
+#[local] Open Scope R_scope.
 
 Definition pr_dist (X Y : expr)
   (σ σ' : state) (v : val) : nonnegreal.
@@ -12,7 +13,7 @@ Proof.
 Defined.
 
 Fact pr_dist_triangle' X Y Z σ σ' σ'' v :
-  (pr_dist X Z σ σ'' v <= (pr_dist X Y σ σ' v) + (pr_dist Y Z σ' σ'' v))%R.
+  (pr_dist X Z σ σ'' v <= (pr_dist X Y σ σ' v) + (pr_dist Y Z σ' σ'' v)).
 Proof.
   rewrite /pr_dist. etrans. 2: apply Rabs_triang. right. simpl. f_equal. lra.
 Qed.
@@ -21,15 +22,14 @@ Fact pr_dist_triangle X Y Z v ε1 ε2 ε3 :
   ((∀ σ σ', pr_dist X Y σ σ' v <= ε1) →
    (∀ σ σ', pr_dist Y Z σ σ' v <= ε2) →
    (ε1 + ε2 <= ε3) →
-   ∀ σ σ', pr_dist X Z σ σ' v <= ε3)%R.
+   ∀ σ σ', pr_dist X Z σ σ' v <= ε3).
 Proof.
   intros. etrans.
   1: eapply (pr_dist_triangle' _ Y _ _ σ).
-  etrans. 2: eauto.
-  apply Rplus_le_compat => //.
+  etrans. 2: eauto. apply Rplus_le_compat => //.
 Qed.
 
-Definition pr_dist_st X Y v := (λ ε : R, ∃ (σ σ' : state), nonneg (pr_dist X Y σ σ' v) = ε)%R.
+Definition pr_dist_st X Y v := (λ ε : R, ∃ (σ σ' : state), nonneg (pr_dist X Y σ σ' v) = ε).
 
 Fact pr_dist_st_bound X Y v : bound (pr_dist_st X Y v).
 Proof.
@@ -40,8 +40,7 @@ Proof.
 Qed.
 
 Fact pr_dist_st_inhabited : forall X Y v, (∃ x : R, pr_dist_st X Y v x).
-  intros.
-  rewrite /pr_dist_st.
+  intros. rewrite /pr_dist_st.
   exists (pr_dist X Y inhabitant inhabitant v) , inhabitant , inhabitant => //.
 Qed.
 
@@ -63,14 +62,12 @@ Definition advantage (X Y : expr) (v : val) : nonnegreal.
 Defined.
 
 Lemma advantage_uniform (X Y : expr) v (ε : R) :
-  (∀ (σ σ' : state), pr_dist X Y σ σ' v <= ε)%R →
-  (advantage X Y v <= ε)%R.
+  (∀ (σ σ' : state), pr_dist X Y σ σ' v <= ε) →
+  (advantage X Y v <= ε).
 Proof.
-  intros hε.
-  rewrite /advantage/advantage_R => /=.
+  intros hε. rewrite /advantage/advantage_R => /=.
   destruct completeness as [x [ub lub]] => /=.
-  apply lub.
-  intros ε' (σ & σ' & hε').
+  apply lub. intros ε' (σ & σ' & hε').
   rewrite -hε'. apply hε.
 Qed.
 
@@ -82,10 +79,9 @@ Proof.
 Qed.
 
 Fact advantage_triangle' X Y Z v :
-  (advantage X Z v <= (advantage X Y v) + (advantage Y Z v))%R.
+  (advantage X Z v <= (advantage X Y v) + (advantage Y Z v)).
 Proof.
-  apply advantage_uniform.
-  intros.
+  apply advantage_uniform. intros.
   transitivity (pr_dist X Y σ σ' v + (pr_dist Y Z σ' σ' v)).
   1: apply pr_dist_triangle'.
   eapply Rplus_le_compat => //.
@@ -96,7 +92,7 @@ Fact advantage_triangle X Y Z v ε1 ε2 ε3 :
   ((advantage X Y v <= ε1) →
    (advantage Y Z v <= ε2) →
    (ε1 + ε2 <= ε3) →
-   advantage X Z v <= ε3)%R.
+   advantage X Z v <= ε3).
 Proof.
   intros. etrans.
   1: eapply (advantage_triangle' _ Y _ _).
